# practice #5.1

* 5

$$\frac {17-2}{-4-(-1)}$$

$$\frac {15}{-3}$$

$$\frac {15}{-3}$$

$$-5$$

* 27

$$y - (-1) = 2(x - 0)$$

$$y + 1 = 2x$$

$$y = 2x -1$$

![image](https://github.com/user-attachments/assets/dd96d475-0bd4-422f-92f1-0a63fc2e947b)

* 43

$$24x + 40y = 15$$

$$40y = -24x + 15$$

$$y = -\frac{24}{40}x + \frac {15}{40}$$

$$\frac {\frac {15}{5}}{\frac {40}{5}} = \frac {3}{8} $$

$$y = -\frac{3}{5}x + \frac {3}{8}$$

![image](https://github.com/user-attachments/assets/f7115c11-0ea5-4229-9c69-2704ee661d6e)


# practice #5.2

* 5

$$x = 4, y = -1$$

$$x - y = 5$$

$$4 - (-1) = 5$$

$$4 +1 = 5$$

$$5 = 5$$


$$2x + y = 7$$

$$2(4) + (-1) = 7$$

$$8 + (-1) = 7$$

$$7 = 7$$

**Yes (4,-1) is a solution for both equations**

* 15

![image](https://github.com/user-attachments/assets/e5275276-9884-433c-a1f1-5a1c17665f22)


**(3,0) is the solution**

# practice #5.3

* 5

$$x = y + 3$$

$$x - 2y = 5$$

$$x = 2y + 5$$

$$(2y + 5) = y + 3$$

$$2y = y -2$$

$$y = -2$$

$$y = -2$$

$$x = 2(-2) + 5$$

$$x = -4 + 5$$

$$x = 1$$

**x,y = (1,-2)**

* 13

$$33x + 2y = 34$$

$$40y = 9x + 11$$

$$y = \frac {9x + 11}{40}$$

$$33x + 2*\frac {9x + 11}{40} = 34$$

$$40(33x) + 18x + 22 = 40(34)$$

$$1320x + 18x + 22 = 1360$$

$$1338x = 1338$$

$$x = 1$$

$$40y = 9(1) + 11$$

$$40y = 20$$

$$y = \frac {1}{2}$$

**x,y = (1,1/2)**

* 15

$$x + 2y = 5$$

$$x - 2y = 1$$

$$x + x = 5 + 1$$

$$2x = 6$$

$$x = 3$

$$3 - 2y = 1$$

$$- 2y = -2$$

$$y = 1$$

**x,y = (3,1)**

* 21

$$v + 2t = 7$$

$$2v + 4t = 9$$

$$-2v -4t = -14$$

$$2v + -2v = 9+14$$

$$0 = 21$$

**There are no solutions**

* 23

$$2x -3y -4 = 0$$

$$3x + 2 = 2y$$

$$2x -3y = 4$$

$$3x + -2y = -2$$

$$6x -9y = 12$$

$$-6x + 4y = 4$$

$$-9y + 4y = 12 + 4$$

$$-5y = 16$$

$$y = \frac {-16}{5}$$

$$3x + 2 = 2(\frac {-16}{5})$$

$$3x + 2 = \frac {-32}{5}$$

$$3x = \frac {-42}{5}$$

$$x = \frac {-14}{5}$$

**x,y = (-14/5, -16/5)**

* 43

$$v1 + v2 = 15v$$

$$v1 - v2 = 3v$$

$$2(v1) = 18v$$


$$v1 = 9v$$

$$v2 + 9v = 15v$$

$$v2 = 6v$$

**v1,v2 = (9v,6v)**

* 53

# 6.2

* 9

$$15x^2 -3x$$

$$3x(5x -1)$$

* 19

$$6pq^2 - 5pq - 14pq^3$$

$$pq(6q -5 -12q^2)$$

* 23

$$x^2 - 9$$

$$(x -3)(x + 3)$$

* 26

$$49 - z^4$$

$$(z^2 - 7)(z^2 + 7)$$

* 33

$$(x + y)^2 - 9$$

$$(x + y - 3)(x + y + 3)$$

* 35

$$32 -18x^2$$

$$2(4 - 3x)(4 + 3x)$$

* 49

$$3 - 2s = 2(3 - st)$$

$$3 - 2s = 6 -2st$$

$$-3 - 2s = -2st$$

$$\frac {-3 - 2s}{-2t} = s$$

$$s = \frac {-3 - 2s}{-2t}$$

# 6.3

* 5

$$x^2 + 6x + 5$$

$$(x + 1) (x + 5)$$

* 7

$$s^2 -s -56$$

$$(s + 7)(s -8)$$

* 11

$$x^2 + 2x + 1$$

$$(x + 1)^2$$

* 13

$$L^2 - 4LK + 4K^2$$

$$a^2 - 2ab + b^2 = (a - b)^2$$

$$(L -2K)^2$$

* 15

$$3x^2 -5x -2$$

$$(3x + 1)(x -2)$$

* 17

$$12y^2 -32y -12$$

$$4(3y^2 -8y -3))$$

$$4(3y^2 -8y -3))$$

$$4(3y + 1)(y -3)$$

* 19

$$2s^2 + 13s + 11$$

$$(2s +11)(s + 1)$$

# 6.5

* 29

$$\frac {18x^2y}{24xy}$$

$$\frac {3x}{4}$$

* 31

$$\frac {a + b}{5a^2 + 5ab}$$

$$\frac {a + b}{5a(a + b))}$$

$$\frac {1}{5a)}$$

* 37

$$\frac {3x^2 - 6x}{x - 2}$$


$$\frac {3x(x -2)}{x - 2}$$


$$3x$$

* 41

$$\frac {x^2 -10x + 25}{x^2 - 25}$$

$$\frac {(x-5)^2}{(x-5)(x+5)}$$

$$\frac {(x-5)}{(x+5)}$$

* 45

$$\frac {5x^2 -6x -8}{x^3 + x^2 - 6x}$$

$$\frac {5x^2 -6x -8}{x(x^2 + x + 6)}$$

# 6.6

* 15

$$\frac {2a + 8}{15} \div \frac {a^2 + 8a + 16}{125}$$

$$\frac {2(a + 4)}{15} * \frac {125}{(a + 4)^2}$$

$$\frac {2}{15} * \frac {125}{(a + 4)}$$

$$\frac {50}{3(a + 4)}$$

* 17

$$\frac {x^4 - 9}{x^2} \div (x^2 + 3)^2$$

$$\frac {x^4 - 9}{x^2} * \frac {1}{(x^2 + 3)^2}$$

$$\frac {(x^2 -3)(x^2 +3)}{x^2} * \frac {1}{(x^2 + 3)^2}$$

$$\frac {(x^2 -3)}{x^2(x^2 + 3)}$$

* 23

$$\frac {x^2 + ax}{2b - cx} \div \frac {a^2 + 2ax + x^2}{2bx - cx^2}$$

$$\frac {x^2 + ax}{2b - cx} * \frac {2bx - cx^2}{a^2 + 2ax + x^2}$$

$$\frac {x(x + a)}{1} * \frac {x}{(x + a)^2}$$

$$\frac {x}{1} * \frac {x}{(x + a)}$$

$$\frac {x^2}{x + a}$$
