![image](https://github.com/user-attachments/assets/d7562184-5eec-432a-ae12-9360a0f78e20)

**Not quadratic because there is a term with a degree higher than 2**


![image](https://github.com/user-attachments/assets/8c15d62f-6677-4f58-8678-dcfeaf9e93be)

**Not quadratic because there is a term with a degree higher than 2**

![image](https://github.com/user-attachments/assets/2e59ac5b-fcf0-4124-a7b3-e36ce68c64a3)

**Quadratic**

$$a = 1$$

$$b = 6$$

$$c = -4$$

![image](https://github.com/user-attachments/assets/0cb4348c-4717-416b-9192-ced414b96624)

$$2n^2 -38n = -176$$

$$n =  \frac{-(-38) \pm \sqrt{(-38)^2 -4(2)(176)}}{2(2)}$$

$$n =  \frac{-(-38) \pm \sqrt{36}}{4}$$

**plus**

$$n =  \frac{38 + 6}{4}$$

$$n =  11$$

**minus**

$$n =  \frac{32}{4}$$

$$n =  8$$

![image](https://github.com/user-attachments/assets/ed4efd39-b1bd-421c-88cd-dbf280534478)

$$z^2 -12z + 27 = 0$$

$$z = \frac {-(-12) \pm \sqrt{(-12)^2 - 4(1)(27)}}{2(1)}$$

$$z = \frac {12 \pm \sqrt{144 - 108}}{2}$$

$$z = \frac {12 \pm 6}{2}$$

**plus**

$$z = \frac {12 + 6}{2}$$

$$z = \frac {18}{2}$$

$$z = 9$$

**minus**

$$z = \frac {12 - 6}{2}$$

$$z = \frac {6}{2}$$

$$z = 3$$

![image](https://github.com/user-attachments/assets/79692916-8502-4905-96d1-f1987e795ec4)

$$16x^2 - 25 = 0$$

$$x = \frac {-(0) \pm \sqrt{(0)^2 -4(16)(-25)}}{2(16)}$$

$$x = \frac {0 \pm \sqrt{1600}}{32}$$

$$x = \frac {0 \pm 40}{32}$$

**plus**

$$x = \frac {0 + 40}{32}$$

$$x = \frac {40}{32}$$

$$x = 1.25$$

**minus**

$$x = \frac {0 - 40}{32}$$

$$x = \frac {-40}{32}$$

$$x = -1.25$$

![image](https://github.com/user-attachments/assets/d9fd674e-22c5-413c-8cf8-611faef839ce)

$$b^2 -9 = 0$$

$$b = \frac {-(0) \pm \sqrt{0 - 4(1)(-9)}}{2}$$

$$b = \frac {0 \pm 6}{2}$$

**plus**

$$b = \frac {0 + 6}{2}$$

$$b = 3$$

**minus**

$$b = \frac {0 - 6}{2}$$

$$b = -3$$

![image](https://github.com/user-attachments/assets/467b203e-2e90-4d93-aa63-18ed327e4f74)

$$h = -\frac {b}{2a}$$

$$h = -\frac {4}{2}$$

$$h = -2$$

$$k = (-2)^2 + 4(-2) + 3$$

$$k = 4 + -8 + 3$$

$$k = -1$$

$$vertex = -2,-1$$

**y-intercept**

$$y = 0 + 0 + 3$$

$$y = 0$$

![image](https://github.com/user-attachments/assets/814bf3f0-d323-429f-8c42-2d69ecb9b4f9)


![image](https://github.com/user-attachments/assets/9854fe9d-7372-4086-98c8-6be70ad3d8e7)

$$x^2 + 6x + 5 = 0$$

$$x = \frac {-(6) \pm \sqrt{6^2 - 4(1)(5)}}{2}$$

$$x = \frac {-(6) \pm \sqrt{36 - 20}}{2}$$

$$x = \frac {-(6) \pm \sqrt{16}}{2}$$

$$x = \frac {-(6) \pm 4}{2}$$

**plus**

$$x = \frac {2}{2}$$

$$x = 1$$

**minus**

$$x = \frac {-10}{2}$$

$$x = -5$$

![image](https://github.com/user-attachments/assets/98249514-3ef9-4566-a3c7-f6bc10903c7a)

$$(R+6)(R+2) = 33$$

$$R^2 + 2R +6r + 12 = 33$$

$$R^2 + 8R + 12 = 33$$

$$R^2 + 8R -21 = 0$$

$$R^2 + 8R = 21$$

$$R^2 + 8R + 16 = 21 + 16$$

$$(R + 4)^2 = 36$$

$$R + 4 = \sqrt{37}$$

**final**

$$R = -4 \pm \sqrt{37}$$


