# Formula


* quadratic
```
$$x = \frac {-b \pm \sqrt{b^2 -4ac}} {2a}$$
```
$$x = \frac {-b \pm \sqrt{b^2 -4ac}} {2a}$$

* Example:
$$2x^2 + 3x -2 = 0 $$
##### set up the quadratic formula
$$x = \frac {-(3) \pm \sqrt{(3)^2 -4(2)(-2)}} {2(2)}$$
##### work out the discriminant
$$\sqrt{(3)^2 -4(2)(-2)}$$

$$\sqrt{25}$$
##### plug the discriminant back in
$$x = \frac {-(3) \pm \sqrt{25}} {2(2)}$$
##### plus
$$x = \frac {-(3) + \sqrt{25}} {2(2)}$$

$$x = \frac {-(3) + 5} {4}$$

$$x = \frac {2} {4}$$

$$x = 0.5$$
##### minus
$$x = \frac {-(3) - 5} {2(2)}$$

$$x = \frac {-8} {4}$$

$$x = -2$$
##### answer
$x = 0.5$

$x = -2$

# Factoring


* In standard form:
$$ax^2 + bx + c = 0$$

* In factored form:
$$y = a(x − r)(x − s)$$

### how to factor:


1. Check for Common Factors among the coefficients a,b, and c:
##### example:
$$3x^2 + 6x + 24 = 0$$

$$x^2 + 2x + 8 = 0$$

2. Find factor pairs of $a \times c$: Multiply a and c, then find pairs of numbers that multiply to $a \times c$ and add up to $b$. These pairs will be the coefficients of the factors

3.  Rewrite the middle term bxbx using the factor pairs found in the previous step. Then, group the terms and factor by grouping, or use a common factor between terms if possible.
#### example:
$$y = x^2 -2x -15$$

$$y = (x+3)(x-5)$$

### method for difficult to factor equations:

1. $a \times c$ is the number $r$ and $s$ multiply to. $b$ is the number $r$ and $s$ add to.
2. divide $r$ and $s$ by by $a$
3. the numerator becomes the constant and the denominator becomes the coefficient of $r$ and $s$

##### Example:
$$3x^2 + 10x - 8$$

$num1$ and $num2$ multiply to $-24$ to and $r$ and $s$ add to $10$

$num1 = 12, num2 = -2$

Then we divide by $a$ which is $3$ resulting in $r = \frac {12}{3}, s = \frac {-2}{3}$

Then we simplify resulting in $r = \frac {4}{1}, s = \frac {-2}{3}$

factored form: $(x + 4)(3s -2)$

# Determining Equation From Graph

We can use what we know about the factored form to determine the equation of a quadratic function using certain information about the parabola.  We might start with the graph, or information about the graph.  In order to set up an equation in factored form, we need to know the x-intercepts (this gives us “r” and “s”) and another point on the parabola (this gives us an ordered pair of (x, y) values).  This information will allow us to find the value of “a”.  This is what we need in order to write the full equation.

![PastedImage_l6dhq7wn1df98u4ku7iymnesdeuig8mn0014672063](https://github.com/JackAWatt/jackwatt.com/assets/3372510/b00dcb5a-0b04-4e56-bc49-9b1feec964c6)

By inspection we see a point (4, -4), which happens to be the vertex in this case.  In addition, the x-intercepts give us r = 2 and s = 6.  Therefore, we can substitute what we know into the factored form:

$$y = a(x -r)(x - s)$$

$$-4 = a(4 - 2)(4 - 6)$$

$$-4 = a(2)(-2)$$

$$-4 = -4a$$

$$\frac {-4}{-4} = a$$

$$a = 1$$

Therefore, we can write the equation of the parabola:

$$y = (x -2)(x - 6)$$

or, we can expand to get this in standard form:

$$y = x^2 -6x -2x + 12$$

$$y = x^2 -8x + 12$$

