
* In standard form:
$$ax^2 + bx + c = 0$$

* In factored form:
$$y = a(x − r)(x − s)$$

### how to factor:


1. Check for Common Factors among the coefficients a,b, and c:
##### example:
$$3x^2 + 6x + 24 = 0$$

$$x^2 + 2x + 8 = 0$$

2. Find factor pairs of $a \times c$: Multiply a and c, then find pairs of numbers that multiply to $a \times c$ and add up to $b$. These pairs will be the coefficients of the factors

3.  Rewrite the middle term bxbx using the factor pairs found in the previous step. Then, group the terms and factor by grouping, or use a common factor between terms if possible.
#### example:
$$y = x^2 -2x -15$$

$$y = (x+3)(x-5)$$
