
* quadratic
```
$$x = \frac {-b \pm \sqrt{b^2 -4ac}} {2a}$$
```
$$x = \frac {-b \pm \sqrt{b^2 -4ac}} {2a}$$

* Example:
$$2x^2 + 3x -2 = 0 $$
##### set up the quadratic formula
$$x = \frac {-(3) \pm \sqrt{(3)^2 -4(2)(-2)}} {2(2)}$$
##### work out the discriminant
$$\sqrt{(3)^2 -4(2)(-2)}$$

$$\sqrt{25}$$
##### plug the discriminant back in
$$x = \frac {-(3) \pm \sqrt{25}} {2(2)}$$
##### plus
$$x = \frac {-(3) + \sqrt{25}} {2(2)}$$

$$x = \frac {-(3) + 5} {4}$$

$$x = \frac {2} {4}$$

$$x = 0.5$$
##### minus
$$x = \frac {-(3) - 5} {2(2)}$$

$$x = \frac {-8} {4}$$

$$x = -2$$

