
* In standard form:
$$ax^2 + bx + c = 0$$

* In factored form:
$$y = a(x − r)(x − s)$$

### how to factor:


1. Check for Common Factors among the coefficients a,b, and c:
##### example:
$$3x^2 + 6x + 24 = 0$$

$$x^2 + 2x + 8 = 0$$

2. Find factor pairs of $a \times c$: Multiply a and c, then find pairs of numbers that multiply to $a \times c$ and add up to $b$. These pairs will be the coefficients of the factors

3.  Rewrite the middle term bxbx using the factor pairs found in the previous step. Then, group the terms and factor by grouping, or use a common factor between terms if possible.
#### example:
$$y = x^2 -2x -15$$

$$y = (x+3)(x-5)$$

### method for difficult to factor equations:

1. $a \times c$ is the number $r$ and $s$ multiply to. $b$ is the number $r$ and $s$ add to.
2. divide $r$ and $s$ by by $a$
3. the numerator becomes the constant and the denominator becomes the coefficient of $r$ and $s$

##### Example:
$$3x^2 + 10x - 8$$

$num1$ and $num2$ multiply to $-24$ to and $r$ and $s$ add to $10$

$num1 = 12, num2 = -2$

Then we divide by $a$ which is $3$ resulting in $r = \frac {12}{3}, s = \frac {-2}{3}$

Then we simplify resulting in $r = \frac {4}{1}, s = \frac {-2}{3}$

factored form: $(x + 4)(3s -2)$
